examples/lowparse/LowParse.Examples.Extract.fst
@@ -1,0 +1,8 @@
+module LowParse.Examples.Extract
+open LowParse
+open LowParse.Examples
+
+inline_for_extraction
+let validate_fstar_test
+: stateful_validator parse_fstar_test
+= validate_fstar_test
